Cslib/Computability/Machines/MultiTapeTuring/Routines/Navigation.lean
@@ -17,19 +17,44 @@ namespace Routines
 -- Argument navigation (for Data.list values)
 -- ═══════════════════════════════════════════════════════════════════════════
 
+def skipRight_n {k : ℕ} (n : ℕ) (i : Fin k) : MultiTapeTM k Char :=
+  match n with
+  | 0 => noop
+  | n + 1 => skipRight_n n i ;ₜ skipRight i
+
+@[simp]
+lemma skipRight_n.eval_struct {k : ℕ} {n : ℕ} {i : Fin k} {views : Fin k → TapeView}
+    (path : List ℕ)
+    (h_path : (views i).path = path ++ [idx])
+    (h_hasNextN : ((views i).data.atPath (path ++ [idx + n])).isSome) :
+    (skipRight_n n i).eval_struct views = some
+      (Function.update views i
+        ⟨(views i).data, path ++ [idx + n]⟩) := by
+  induction n generalizing path with
+  | zero => simp [skipRight_n]; ext1 <;> simp [h_path]
+  | succ n ih =>
+    simp [skipRight_n]
+    let ih' := ih path h_path (by sorry)--simp [← Nat.add_assoc] at h_hasNextN; simp [h_hasNextN])
+    rw [ih']
+    simp
+
+
+
+    sorry
+
 /-- Navigate to the `idx`-th element of a `Data.list` encoding on tape `i`.
 Moves past `(` and then skips `idx` Data elements.
 If `i` is larger than the length of the list, does nothing. -/
-public def toElem {k : ℕ} (idx : ℕ) (i : Fin k) : MultiTapeTM k Char := sorry
+public def toElem {k : ℕ} (idx : ℕ) (i : Fin k) : MultiTapeTM k Char :=
+  right i
 
 /-- If positioned on the element of a list, navigates to the list containing it. -/
 public def outOfList {k : ℕ} (i : Fin k) : MultiTapeTM k Char :=
-  -- TOOD what about "not a list"?
-  -- left i ;ₜ while_eq ')' i (right i ;ₜ skipLeft i ;ₜ left i)
-  sorry
+  left i ;ₜ while_eq ')' i (right i ;ₜ skipLeft i ;ₜ left i) ;ₜ
+    -- This part handles the case where we started out with a number on the tape or
+    -- an empty tape.
+    if_eq '(' i noop (right i)
 
--- ((x)()()())
---       ^
 
 /-- `toElem idx i` moves to the `idx`th element of the `Data.list` currently pointed to
 on tape `i`. Only descends if the current element is a `Data.list` with at least `idx` elements,
@@ -38,6 +63,14 @@ otherwise, the `TapeView` is unchanged. -/
 public lemma toElem_eval_struct {k : ℕ} {idx : ℕ} {i : Fin k} {views : Fin k → TapeView} :
   (toElem idx i).eval_struct views = some
     (Function.update views i (((views i).toElem? idx).getD (views i))) := by sorry
+
+-- lemma outOfList_inner {k : ℕ} {i : Fin k} {views : Fin k → TapeView} :
+--   (right i ;ₜ skipLeft i ;ₜ left i).eval (toBiTape ∘ views) =
+--     if (views i).current = some (Data.num 0) then some views else
+--       if (views i).current = some (Data.list []) then some views else
+--         if (views i).current = some (Data.list (_ :: _)) then
+--           some (Function.update views i ⟨(views i).data, (views i).path.dropLast⟩)
+--         else some views := by sorry
 
 /-- `outOfArg argIdx i` ascends back from the `argIdx`-th element,
     removing it from the end of the path. If the path ends with `argIdx`,
