Cslib/Computability/Machines/MultiTapeTuring/StructuralMachines.lean
@@ -9,6 +9,7 @@ module
 public import Cslib.Computability.Machines.MultiTapeTuring.Basic
 public import Cslib.Computability.Machines.MultiTapeTuring.Encoding
 public import Cslib.Computability.Machines.MultiTapeTuring.SequentialCombinator
+public import Mathlib.Data.PFun
 
 namespace Turing
 
@@ -33,16 +34,51 @@ namespace Routines
 -- Primitives
 -- ═══════════════════════════════════════════════════════════════════════════
 
-public def noop : MultiTapeTM k Char := sorry
+variable {Symbol : Type} [Inhabited Symbol] [Fintype Symbol]
+variable {k : ℕ}
+
+public def noop : MultiTapeTM k Symbol := sorry
+
+@[simp]
+public theorem noop.eval_struct {views : Fin k → TapeView} :
+  noop.eval_struct views = some views := by sorry
 
 public def right (i : Fin k) : MultiTapeTM k Char := sorry
 
+@[simp]
+public theorem right.eval {i : Fin k} {tapes : Fin k → BiTape Char} :
+  (right i).eval tapes = some
+    (Function.update tapes i (tapes i).move_right) := by sorry
+
 public def left (i : Fin k) : MultiTapeTM k Char := sorry
+
+@[simp]
+public theorem left.eval {i : Fin k} {tapes : Fin k → BiTape Char} :
+  (left i).eval tapes = some
+    (Function.update tapes i (tapes i).move_left) := by sorry
 
 public def write (c : Char) (i : Fin k) : MultiTapeTM k Char := sorry
 
+public def if_eq (c : Char) (i : Fin k) (tm₁ tm₂ : MultiTapeTM k Char) :
+  MultiTapeTM k Char := sorry
+
+@[simp]
+public theorem if_eq.eval {c : Char} {i : Fin k} {tm₁ tm₂ : MultiTapeTM k Char}
+    {tapes : Fin k → BiTape Char} :
+  (if_eq c i tm₁ tm₂).eval tapes =
+    if (tapes i).head = some c then (tm₁.eval tapes) else (tm₂.eval tapes) := by sorry
+
 public def while_eq (c : Char) (i : Fin k) (tm : MultiTapeTM k Char) :
   MultiTapeTM k Char := sorry
+
+-- @[simp]
+-- public theorem while_eq.eval
+--   (c : Char) (i : Fin k)
+--   (tm : MultiTapeTM k Char)
+--   (tapes : Fin k → BiTape Char) :
+--   (while_eq c i tm).eval tapes =
+--     ⟨∃ n, (((tm.eval)^[n] (.some tapes)) >>= fun tapes => (tapes i).head) = Part.some (some c),
+--     sorry ⟩ := by sorry
 
 public def while_neq (c : Char) (i : Fin k) (tm : MultiTapeTM k Char) :
   MultiTapeTM k Char := sorry
